examples/ghc/manual/DataCon.v
@@ -13,29 +13,19 @@ Require Coq.Program.Wf.
 (* Converted imports: *)
 
 Require BasicTypes.
-Require Class.
 Require Coq.Init.Datatypes.
-Require Coq.Lists.List.
 Require Data.Foldable.
-Require Data.Set.Internal.
-Require Data.Traversable.
 Require Data.Tuple.
-Require FastString.
 Require FieldLabel.
-(* Require ForeignCall. *)
 Require GHC.Base.
 Require GHC.Err.
 Require GHC.List.
 Require GHC.Num.
-Require ListSetOps.
 Require Name.
 Require OccName.
-Require Panic.
-Require PrelNames.
-(* Require TysWiredIn. *)
-Require UniqSet.
+Require TyCon.
 Require Unique.
-Require Util.
+Require Var.
 Import GHC.Base.Notations.
 Import GHC.Num.Notations.
 
@@ -90,7 +80,8 @@ Inductive DataCon : Type
      list FieldLabel.FieldLabel ->
      Var.Id ->
      DataConRep ->
-     BasicTypes.Arity -> BasicTypes.Arity -> unit -> unit -> bool -> unit -> DataCon.
+     BasicTypes.Arity ->
+     BasicTypes.Arity -> TyCon.TyCon -> unit -> bool -> TyCon.TyCon -> DataCon.
 
 Instance Default__StrictnessMark : GHC.Err.Default StrictnessMark :=
   GHC.Err.Build_Default _ MarkedStrict.
@@ -263,50 +254,48 @@ Program Instance Eq___DataCon : GHC.Base.Eq_ DataCon :=
     k {| GHC.Base.op_zeze____ := Eq___DataCon_op_zeze__ ;
          GHC.Base.op_zsze____ := Eq___DataCon_op_zsze__ |}.
 
-(* Translating `instance Uniquable__DataCon' failed: OOPS! Cannot find
-   information for class Qualified "Unique" "Uniquable" unsupported *)
+Local Definition Uniquable__DataCon_getUnique : DataCon -> Unique.Unique :=
+  dcUnique.
 
-(* Translating `instance NamedThing__DataCon' failed: OOPS! Cannot find
-   information for class Qualified "Name" "NamedThing" unsupported *)
+Program Instance Uniquable__DataCon : Unique.Uniquable DataCon :=
+  fun _ k => k {| Unique.getUnique__ := Uniquable__DataCon_getUnique |}.
 
-(* Translating `instance Outputable__DataCon' failed: OOPS! Cannot find
-   information for class Qualified "Outputable" "Outputable" unsupported *)
+Local Definition NamedThing__DataCon_getName : DataCon -> Name.Name :=
+  dcName.
 
-(* Translating `instance OutputableBndr__DataCon' failed: OOPS! Cannot find
-   information for class Qualified "Outputable" "OutputableBndr" unsupported *)
+Local Definition NamedThing__DataCon_getOccName : DataCon -> OccName.OccName :=
+  fun n => Name.nameOccName (NamedThing__DataCon_getName n).
 
-(* Translating `instance Data__DataCon' failed: OOPS! Cannot find information
-   for class Qualified "Data.Data" "Data" unsupported *)
+Program Instance NamedThing__DataCon : Name.NamedThing DataCon :=
+  fun _ k =>
+    k {| Name.getName__ := NamedThing__DataCon_getName ;
+         Name.getOccName__ := NamedThing__DataCon_getOccName |}.
 
-(* Translating `instance Outputable__EqSpec' failed: OOPS! Cannot find
-   information for class Qualified "Outputable" "Outputable" unsupported *)
+(* Skipping instance Outputable__DataCon of class Outputable *)
 
-(* Translating `instance Outputable__StrictnessMark' failed: OOPS! Cannot find
-   information for class Qualified "Outputable" "Outputable" unsupported *)
+(* Skipping instance OutputableBndr__DataCon of class OutputableBndr *)
 
-(* Translating `instance Outputable__HsSrcBang' failed: OOPS! Cannot find
-   information for class Qualified "Outputable" "Outputable" unsupported *)
+(* Skipping instance Data__DataCon of class Data *)
 
-(* Translating `instance Outputable__SrcUnpackedness' failed: OOPS! Cannot find
-   information for class Qualified "Outputable" "Outputable" unsupported *)
+(* Skipping instance Outputable__EqSpec of class Outputable *)
 
-(* Translating `instance Binary__SrcUnpackedness' failed: OOPS! Cannot find
-   information for class Qualified "Binary" "Binary" unsupported *)
+(* Skipping instance Outputable__StrictnessMark of class Outputable *)
 
-(* Translating `instance Outputable__SrcStrictness' failed: OOPS! Cannot find
-   information for class Qualified "Outputable" "Outputable" unsupported *)
+(* Skipping instance Outputable__HsSrcBang of class Outputable *)
 
-(* Translating `instance Binary__SrcStrictness' failed: OOPS! Cannot find
-   information for class Qualified "Binary" "Binary" unsupported *)
+(* Skipping instance Outputable__SrcUnpackedness of class Outputable *)
 
-(* Translating `instance Outputable__HsImplBang' failed: OOPS! Cannot find
-   information for class Qualified "Outputable" "Outputable" unsupported *)
+(* Skipping instance Binary__SrcUnpackedness of class Binary *)
 
-(* Translating `instance Data__HsSrcBang' failed: OOPS! Cannot find information
-   for class Qualified "Data.Data" "Data" unsupported *)
+(* Skipping instance Outputable__SrcStrictness of class Outputable *)
 
-(* Translating `instance Data__SrcUnpackedness' failed: OOPS! Cannot find
-   information for class Qualified "Data.Data" "Data" unsupported *)
+(* Skipping instance Binary__SrcStrictness of class Binary *)
+
+(* Skipping instance Outputable__HsImplBang of class Outputable *)
+
+(* Skipping instance Data__HsSrcBang of class Data *)
+
+(* Skipping instance Data__SrcUnpackedness of class Data *)
 
 Local Definition Eq___SrcUnpackedness_op_zeze__
    : SrcUnpackedness -> SrcUnpackedness -> bool :=
@@ -327,8 +316,7 @@ Program Instance Eq___SrcUnpackedness : GHC.Base.Eq_ SrcUnpackedness :=
     k {| GHC.Base.op_zeze____ := Eq___SrcUnpackedness_op_zeze__ ;
          GHC.Base.op_zsze____ := Eq___SrcUnpackedness_op_zsze__ |}.
 
-(* Translating `instance Data__SrcStrictness' failed: OOPS! Cannot find
-   information for class Qualified "Data.Data" "Data" unsupported *)
+(* Skipping instance Data__SrcStrictness of class Data *)
 
 Local Definition Eq___SrcStrictness_op_zeze__
    : SrcStrictness -> SrcStrictness -> bool :=
@@ -349,40 +337,7 @@ Program Instance Eq___SrcStrictness : GHC.Base.Eq_ SrcStrictness :=
     k {| GHC.Base.op_zeze____ := Eq___SrcStrictness_op_zeze__ ;
          GHC.Base.op_zsze____ := Eq___SrcStrictness_op_zsze__ |}.
 
-(* Translating `instance Data__HsImplBang' failed: OOPS! Cannot find information
-   for class Qualified "Data.Data" "Data" unsupported *)
-
-(*
-Definition buildAlgTyCon
-   : Name.Name ->
-     list Var.TyVar ->
-     list CoAxiom.Role ->
-     option unit ->
-     unit -> TyCon.AlgTyConRhs -> bool -> unut -> unit := tt.
-  fun tc_name ktvs roles cType stupid_theta rhs gadt_syn parent => tt.
-    let binders := Type.mkTyConBindersPreferAnon ktvs TysWiredIn.liftedTypeKind in
-    TyCon.mkAlgTyCon tc_name binders TysWiredIn.liftedTypeKind roles cType
-    stupid_theta rhs parent gadt_syn. 
-
-Definition buildSynTyCon
-   : Name.Name ->
-     list TyCon.TyConBinder -> unit -> list CoAxiom.Role -> unit -> unit :=
-  fun name binders res_kind roles rhs =>
-    let is_fam_free := Type.isFamFreeTy rhs in
-    let is_tau := Type.isTauTy rhs in
-    TyCon.mkSynonymTyCon name binders res_kind roles rhs is_tau is_fam_free.
-*)
-
-Definition classDataCon : Class.Class -> DataCon :=
-  fun clas =>
-    match TyCon.tyConDataCons (Class.classTyCon clas) with
-    | cons dict_constr no_more =>
-        if andb Util.debugIsOn (negb (Data.Foldable.null no_more)) : bool
-        then (Panic.assertPanic (GHC.Base.hs_string__
-                                 "ghc/compiler/basicTypes/DataCon.hs") #1346)
-        else dict_constr
-    | nil => Panic.panic (GHC.Base.hs_string__ "classDataCon")
-    end.
+(* Skipping instance Data__HsImplBang of class Data *)
 
 Definition dataConBoxer : DataCon -> option unit :=
   fun arg_0__ =>
@@ -392,14 +347,6 @@ Definition dataConBoxer : DataCon -> option unit :=
     | _ => None
     end.
 
-Definition dataConExTyVars : DataCon -> list Var.TyVar :=
-  fun arg_0__ =>
-    let 'MkData _ _ _ _ _ tvbs _ _ _ _ _ _ _ _ _ _ _ _ _ _ _ _ := arg_0__ in
-    tvbs.
-
-Definition dataConFieldLabels : DataCon -> list FieldLabel.FieldLabel :=
-  dcFields.
-
 Definition dataConFieldType_maybe
    : DataCon ->
      FieldLabel.FieldLabelString -> option (FieldLabel.FieldLabel * unit)%type :=
@@ -407,15 +354,6 @@ Definition dataConFieldType_maybe
     Data.Foldable.find ((fun arg_0__ => arg_0__ GHC.Base.== label) GHC.Base.∘
                         (FieldLabel.flLabel GHC.Base.∘ Data.Tuple.fst)) (GHC.List.zip (dcFields con)
                                                                                       (dcOrigArgTys con)).
-
-Definition dataConFieldType : DataCon -> FieldLabel.FieldLabelString -> unit :=
-  fun con label =>
-    match dataConFieldType_maybe con label with
-    | Some (pair _ ty) => ty
-    | None =>
-        Panic.panicStr (GHC.Base.hs_string__ "dataConFieldType") (GHC.Base.mappend
-                                                                  (Panic.noString con) (Panic.noString label))
-    end.
 
 Definition dataConFullSig
    : DataCon ->
@@ -433,111 +371,11 @@ Definition dataConImplBangs : DataCon -> list HsImplBang :=
     | DCR _ _ _ _ bangs => bangs
     end.
 
-Definition dataConImplicitTyThings : DataCon -> list unit :=
-  fun arg_0__ =>
-    let 'MkData _ _ _ _ _ _ _ _ _ _ _ _ _ _ work rep _ _ _ _ _ _ := arg_0__ in
-    let wrap_ids :=
-      match rep with
-      | NoDataConRep => nil
-      | DCR wrap _ _ _ _ => cons (TyCoRep.AnId wrap) nil
-      end in
-    Coq.Init.Datatypes.app (cons (TyCoRep.AnId work) nil) wrap_ids.
-
-Definition dataConInstOrigArgTys : DataCon -> list unit -> list unit :=
-  fun arg_0__ arg_1__ =>
-    match arg_0__, arg_1__ with
-    | (MkData _ _ _ _ univ_tvs ex_tvs _ _ _ _ arg_tys _ _ _ _ _ _ _ _ _ _ _ as dc)
-    , inst_tys =>
-        let tyvars := Coq.Init.Datatypes.app univ_tvs ex_tvs in
-        if andb Util.debugIsOn (negb (Util.equalLength tyvars inst_tys)) : bool
-        then (Outputable.assertPprPanic (GHC.Base.hs_string__
-                                         "ghc/compiler/basicTypes/DataCon.hs") #1274 ((GHC.Base.mappend (id
-                                                                                                         (GHC.Base.hs_string__
-                                                                                                          "dataConInstOrigArgTys"))
-                                                                                                        (Panic.noString
-                                                                                                         dc)
-                                                                                       Outputable.$$
-                                                                                       Panic.noString tyvars)
-                                                                                      Outputable.$$
-                                                                                      Panic.noString inst_tys))
-        else GHC.Base.map (TyCoRep.substTyWith tyvars inst_tys) arg_tys
-    end.
-
 Definition dataConIsInfix : DataCon -> bool :=
   dcInfix.
 
 Definition dataConName : DataCon -> Name.Name :=
   dcName.
-
-Definition dataConOrigArgTys : DataCon -> list unit :=
-  fun dc => dcOrigArgTys dc.
-
-Definition dataConOrigResTy : DataCon -> unit :=
-  fun dc => dcOrigResTy dc.
-
-Definition dataConOrigTyCon : DataCon -> unit :=
-  fun dc =>
-    match TyCon.tyConFamInst_maybe (dcRepTyCon dc) with
-    | Some (pair tc _) => tc
-    | _ => dcRepTyCon dc
-    end.
-
-Definition dataConRepArgTys : DataCon -> list unit :=
-  fun arg_0__ =>
-    let 'MkData _ _ _ _ _ _ _ eq_spec theta _ orig_arg_tys _ _ _ _ rep _ _ _ _ _
-       _ := arg_0__ in
-    match rep with
-    | NoDataConRep =>
-        if andb Util.debugIsOn (negb (Data.Foldable.null eq_spec)) : bool
-        then (Panic.assertPanic (GHC.Base.hs_string__
-                                 "ghc/compiler/basicTypes/DataCon.hs") #1293)
-        else Coq.Init.Datatypes.app theta orig_arg_tys
-    | DCR _ _ arg_tys _ _ => arg_tys
-    end.
-
-Definition dataConRepStrictness : DataCon -> list StrictnessMark :=
-  fun dc =>
-    match dcRep dc with
-    | NoDataConRep =>
-        Coq.Lists.List.flat_map (fun _ => cons NotMarkedStrict nil) (dataConRepArgTys
-                                 dc)
-    | DCR _ _ _ strs _ => strs
-    end.
-
-Definition dataConInstArgTys : DataCon -> list unit -> list unit :=
-  fun arg_0__ arg_1__ =>
-    match arg_0__, arg_1__ with
-    | (MkData _ _ _ _ univ_tvs ex_tvs _ _ _ _ _ _ _ _ _ _ _ _ _ _ _ _ as dc)
-    , inst_tys =>
-        if andb Util.debugIsOn (negb (Util.equalLength univ_tvs inst_tys)) : bool
-        then (Outputable.assertPprPanic (GHC.Base.hs_string__
-                                         "ghc/compiler/basicTypes/DataCon.hs") #1257 ((GHC.Base.mappend (id
-                                                                                                         (GHC.Base.hs_string__
-                                                                                                          "dataConInstArgTys"))
-                                                                                                        (Panic.noString
-                                                                                                         dc)
-                                                                                       Outputable.$$
-                                                                                       Panic.noString univ_tvs)
-                                                                                      Outputable.$$
-                                                                                      Panic.noString inst_tys))
-        else if andb Util.debugIsOn (negb (Data.Foldable.null ex_tvs)) : bool
-             then (Outputable.assertPprPanic (GHC.Base.hs_string__
-                                              "ghc/compiler/basicTypes/DataCon.hs") #1258 (Panic.noString dc))
-             else GHC.Base.map (TyCoRep.substTyWith univ_tvs inst_tys) (dataConRepArgTys dc)
-    end.
-
-Definition splitDataProductType_maybe
-   : unit -> option (unit * list unit * DataCon * list unit)%type :=
-  fun ty =>
-    match Type.splitTyConApp_maybe ty with
-    | Some (pair tycon ty_args) =>
-        match TyCon.isDataProductTyCon_maybe tycon with
-        | Some con =>
-            Some (pair (pair (pair tycon ty_args) con) (dataConInstArgTys con ty_args))
-        | _ => None
-        end
-    | _ => None
-    end.
 
 Definition dataConRepArity : DataCon -> BasicTypes.Arity :=
   fun arg_0__ =>
@@ -570,11 +408,8 @@ Definition dataConTag : DataCon -> BasicTypes.ConTag :=
 Definition dataConTagZ : DataCon -> BasicTypes.ConTagZ :=
   fun con => dataConTag con GHC.Num.- BasicTypes.fIRST_TAG.
 
-Definition dataConTyCon : DataCon -> unit :=
+Definition dataConTyCon : DataCon -> TyCon.TyCon :=
   dcRepTyCon.
-
-Definition specialPromotedDc : DataCon -> bool :=
-  TyCon.isKindTyCon GHC.Base.∘ dataConTyCon.
 
 Definition dataConUnivAndExTyVars : DataCon -> list Var.TyVar :=
   fun arg_0__ =>
@@ -595,13 +430,6 @@ Definition dataConUserTyVars : DataCon -> list Var.TyVar :=
     let 'MkData _ _ _ _ _ _ tvbs _ _ _ _ _ _ _ _ _ _ _ _ _ _ _ := arg_0__ in
     Var.binderVars tvbs.
 
-Definition dataConUserType : DataCon -> unit :=
-  fun arg_0__ =>
-    let 'MkData _ _ _ _ _ _ user_tvbs _ theta _ arg_tys res_ty _ _ _ _ _ _ _ _ _
-       _ := arg_0__ in
-    TyCoRep.mkForAllTys user_tvbs (TyCoRep.mkFunTys theta (TyCoRep.mkFunTys arg_tys
-                                                                            res_ty)).
-
 Definition dataConWorkId : DataCon -> Var.Id :=
   fun dc => dcWorkId dc.
 
@@ -619,68 +447,8 @@ Definition dataConWrapId_maybe : DataCon -> option Var.Id :=
     | DCR wrap_id _ _ _ _ => Some wrap_id
     end.
 
-Definition eqHsBang : HsImplBang -> HsImplBang -> bool :=
-  fun arg_0__ arg_1__ =>
-    match arg_0__, arg_1__ with
-    | HsLazy, HsLazy => true
-    | HsStrict, HsStrict => true
-    | HsUnpack None, HsUnpack None => true
-    | HsUnpack (Some c1), HsUnpack (Some c2) =>
-        Type.eqType (Coercion.coercionType c1) (Coercion.coercionType c2)
-    | _, _ => false
-    end.
-
 Definition eqSpecPair : EqSpec -> (Var.TyVar * unit)%type :=
   fun arg_0__ => let 'Mk_EqSpec tv ty := arg_0__ in pair tv ty.
-
-Definition eqSpecPreds : list EqSpec -> unit :=
-  fun spec =>
-    let cont_0__ arg_1__ :=
-      let 'Mk_EqSpec tv ty := arg_1__ in
-      cons (Type.mkPrimEqPred (TyCoRep.mkTyVarTy tv) ty) nil in
-    Coq.Lists.List.flat_map cont_0__ spec.
-
-Definition dataConTheta : DataCon -> unit :=
-  fun arg_0__ =>
-    let 'MkData _ _ _ _ _ _ _ eq_spec theta _ _ _ _ _ _ _ _ _ _ _ _ _ := arg_0__ in
-    Coq.Init.Datatypes.app (eqSpecPreds eq_spec) theta.
-
-Definition dataConSig
-   : DataCon -> (list Var.TyVar * unit * list unit * unit)%type :=
-  fun arg_0__ =>
-    let '(MkData _ _ _ _ _ _ _ _ _ _ arg_tys res_ty _ _ _ _ _ _ _ _ _ _ as con) :=
-      arg_0__ in
-    pair (pair (pair (dataConUnivAndExTyVars con) (dataConTheta con)) arg_tys)
-         res_ty.
-
-Definition dataConInstSig
-   : DataCon -> list unit -> (list Var.TyVar * unit * list unit)%type :=
-  fun arg_0__ arg_1__ =>
-    match arg_0__, arg_1__ with
-    | MkData _ _ _ _ univ_tvs ex_tvs _ eq_spec theta _ arg_tys _ _ _ _ _ _ _ _ _ _ _
-    , univ_tys =>
-        let univ_subst := TyCoRep.zipTvSubst univ_tvs univ_tys in
-        let 'pair subst ex_tvs' := Data.Traversable.mapAccumL TyCoRep.substTyVarBndr
-                                     univ_subst ex_tvs in
-        pair (pair ex_tvs' (TyCoRep.substTheta subst (Coq.Init.Datatypes.app
-                                                      (eqSpecPreds eq_spec) theta))) (TyCoRep.substTys subst arg_tys)
-    end.
-
-Definition dataConCannotMatch : list unit -> DataCon -> bool :=
-  fun tys con =>
-    let predEqs :=
-      fun pred =>
-        match Type.classifyPredType pred with
-        | Type.EqPred Type.NomEq ty1 ty2 => cons (pair ty1 ty2) nil
-        | Type.ClassPred eq (cons _ (cons ty1 (cons ty2 nil))) =>
-            if Unique.hasKey eq PrelNames.eqTyConKey : bool
-            then cons (pair ty1 ty2) nil else
-            nil
-        end in
-    let 'pair (pair _ inst_theta) _ := dataConInstSig con tys in
-    if Data.Foldable.null inst_theta : bool then false else
-    if Data.Foldable.all Type.isTyVarTy tys : bool then false else
-    Unify.typesCantMatch (Data.Foldable.concatMap predEqs inst_theta).
 
 Definition eqSpecTyVar : EqSpec -> Var.TyVar :=
   fun arg_0__ => let 'Mk_EqSpec tv _ := arg_0__ in tv.
@@ -703,118 +471,6 @@ Definition dataConUserTyVarsArePermuted : DataCon -> bool :=
 Definition eqSpecType : EqSpec -> unit :=
   fun arg_0__ => let 'Mk_EqSpec _ ty := arg_0__ in ty.
 
-Definition freshNames : list Name.Name -> list Name.Name :=
-  fun avoids =>
-    let avoid_occs : OccName.OccSet :=
-      OccName.mkOccSet (GHC.Base.map Name.getOccName avoids) in
-    let avoid_uniqs : UniqSet.UniqSet Unique.Unique :=
-      UniqSet.mkUniqSet (GHC.Base.map Unique.getUnique avoids) in
-    Coq.Lists.List.flat_map (fun n =>
-                               let occ :=
-                                 OccName.mkTyVarOccFS (FastString.mkFastString (cons (GHC.Char.hs_char__ "x")
-                                                                                     (GHC.Show.show n))) in
-                               let uniq := Unique.mkAlphaTyVarUnique n in
-                               if negb (UniqSet.elementOfUniqSet uniq avoid_uniqs) : bool
-                               then if negb (OccName.elemOccSet occ avoid_occs) : bool
-                                    then cons (Name.mkSystemName uniq occ) nil else
-                                    nil else
-                               nil) (enumFrom #0).
-
-Definition mkCleanAnonTyConBinders
-   : list TyCon.TyConBinder -> list unit -> list TyCon.TyConBinder :=
-  fun tc_bndrs tys =>
-    let fresh_names :=
-      freshNames (GHC.Base.map Name.getName (Var.binderVars tc_bndrs)) in
-    let cont_1__ arg_2__ :=
-      let 'pair name ty := arg_2__ in
-      cons (TyCon.mkAnonTyConBinder (Var.mkTyVar name ty)) nil in
-    Coq.Lists.List.flat_map cont_1__ (GHC.List.zip fresh_names tys).
-
-Definition mkDataCon
-   : Name.Name ->
-     bool ->
-     TyCon.TyConRepName ->
-     list HsSrcBang ->
-     list FieldLabel.FieldLabel ->
-     list Var.TyVar ->
-     list Var.TyVar ->
-     list Var.TyVarBinder ->
-     list EqSpec ->
-     unit ->
-     list unit ->
-     unit ->
-     TyCon.RuntimeRepInfo -> unit -> unit -> Var.Id -> DataConRep -> DataCon :=
-  fun name
-  declared_infix
-  prom_info
-  arg_stricts
-  fields
-  univ_tvs
-  ex_tvs
-  user_tvbs
-  eq_spec
-  theta
-  orig_arg_tys
-  orig_res_ty
-  rep_info
-  rep_tycon
-  stupid_theta
-  work_id
-  rep =>
-    let roles :=
-      Coq.Init.Datatypes.app (GHC.Base.map (GHC.Base.const CoAxiom.Nominal)
-                              (Coq.Init.Datatypes.app univ_tvs ex_tvs)) (GHC.Base.map (GHC.Base.const
-                                                                                       CoAxiom.Representational)
-                              orig_arg_tys) in
-    let prom_res_kind := orig_res_ty in
-    let user_tvbs_invariant :=
-      Data.Set.Internal.fromList (Coq.Init.Datatypes.app (filterEqSpec eq_spec
-                                                          univ_tvs) ex_tvs) GHC.Base.==
-      Data.Set.Internal.fromList (Var.binderVars user_tvbs) in
-    let user_tvbs' :=
-      if andb Util.debugIsOn (negb (user_tvbs_invariant)) : bool
-      then (Outputable.assertPprPanic (GHC.Base.hs_string__
-                                       "ghc/compiler/basicTypes/DataCon.hs") #897 ((Panic.noString univ_tvs
-                                                                                    Outputable.$$
-                                                                                    Panic.noString ex_tvs) Outputable.$$
-                                                                                   Panic.noString user_tvbs))
-      else user_tvbs in
-    let prom_tv_bndrs :=
-      let cont_3__ arg_4__ :=
-        match arg_4__ with
-        | Var.TvBndr tv vis => cons (TyCon.mkNamedTyConBinder vis tv) nil
-        | _ => nil
-        end in
-      Coq.Lists.List.flat_map cont_3__ user_tvbs' in
-    let prom_arg_bndrs :=
-      mkCleanAnonTyConBinders prom_tv_bndrs (Coq.Init.Datatypes.app theta
-                                                                    orig_arg_tys) in
-    let is_vanilla :=
-      andb (Data.Foldable.null ex_tvs) (andb (Data.Foldable.null eq_spec)
-                                             (Data.Foldable.null theta)) in
-    let con :=
-      MkData name (Name.nameUnique name) tag is_vanilla univ_tvs ex_tvs user_tvbs'
-             eq_spec theta stupid_theta orig_arg_tys orig_res_ty arg_stricts fields work_id
-             rep (Data.Foldable.length rep_arg_tys) (Data.Foldable.length orig_arg_tys)
-             rep_tycon rep_ty declared_infix promoted in
-    let tag :=
-      ListSetOps.assoc (GHC.Base.hs_string__ "mkDataCon") (GHC.List.zip
-                                                           (TyCon.tyConDataCons rep_tycon) (enumFrom
-                                                            BasicTypes.fIRST_TAG)) con in
-    let rep_arg_tys := dataConRepArgTys con in
-    let rep_ty :=
-      match rep with
-      | NoDataConRep => dataConUserType con
-      | DCR _ _ _ _ _ =>
-          Type.mkInvForAllTys univ_tvs (Type.mkInvForAllTys ex_tvs (TyCoRep.mkFunTys
-                                                             rep_arg_tys (Type.mkTyConApp rep_tycon (TyCoRep.mkTyVarTys
-                                                                                           univ_tvs))))
-      end in
-    let promoted :=
-      TyCon.mkPromotedDataCon con name prom_info (Coq.Init.Datatypes.app prom_tv_bndrs
-                                                                         prom_arg_bndrs) prom_res_kind roles rep_info in
-    con.
-
 Definition isBanged : HsImplBang -> bool :=
   fun arg_0__ =>
     match arg_0__ with
@@ -822,11 +478,6 @@ Definition isBanged : HsImplBang -> bool :=
     | HsStrict => true
     | HsLazy => false
     end.
-
-Definition isLegacyPromotableTyCon : unit -> bool :=
-  fun tc =>
-    orb (TyCon.isVanillaAlgTyCon tc) (orb (TyCon.isFunTyCon tc) (TyCon.isKindTyCon
-                                           tc)).
 
 Definition isMarkedStrict : StrictnessMark -> bool :=
   fun arg_0__ => match arg_0__ with | NotMarkedStrict => false | _ => true end.
@@ -858,118 +509,22 @@ Definition isVanillaDataCon : DataCon -> bool :=
 Definition mkEqSpec : Var.TyVar -> unit -> EqSpec :=
   fun tv ty => Mk_EqSpec tv ty.
 
-Definition dataConEqSpec : DataCon -> list EqSpec :=
-  fun arg_0__ =>
-    let 'MkData _ _ _ _ _ _ _ eq_spec theta _ _ _ _ _ _ _ _ _ _ _ _ _ := arg_0__ in
-    Coq.Init.Datatypes.app eq_spec (Coq.Init.Datatypes.app (let cont_1__ arg_2__ :=
-                                                              match arg_2__ with
-                                                              | Some (pair tc (cons _k1 (cons _k2 (cons ty1 (cons ty2
-                                                                   nil))))) =>
-                                                                  if Unique.hasKey tc PrelNames.heqTyConKey : bool
-                                                                  then Coq.Lists.List.flat_map (fun spec =>
-                                                                                                  cons spec nil)
-                                                                                               (match pair
-                                                                                                        (Type.getTyVar_maybe
-                                                                                                         ty1)
-                                                                                                        (Type.getTyVar_maybe
-                                                                                                         ty2) with
-                                                                                                | pair (Some tv1) _ =>
-                                                                                                    cons (mkEqSpec tv1
-                                                                                                          ty2) nil
-                                                                                                | pair _ (Some tv2) =>
-                                                                                                    cons (mkEqSpec tv2
-                                                                                                          ty1) nil
-                                                                                                | _ => nil
-                                                                                                end) else
-                                                                  nil
-                                                              | _ => nil
-                                                              end in
-                                                            Coq.Lists.List.flat_map cont_1__ (GHC.Base.map
-                                                                                     Type.splitTyConApp_maybe theta))
-                                                           (let cont_7__ arg_8__ :=
-                                                              match arg_8__ with
-                                                              | Some (pair tc (cons _k (cons ty1 (cons ty2 nil)))) =>
-                                                                  if Unique.hasKey tc PrelNames.eqTyConKey : bool
-                                                                  then Coq.Lists.List.flat_map (fun spec =>
-                                                                                                  cons spec nil)
-                                                                                               (match pair
-                                                                                                        (Type.getTyVar_maybe
-                                                                                                         ty1)
-                                                                                                        (Type.getTyVar_maybe
-                                                                                                         ty2) with
-                                                                                                | pair (Some tv1) _ =>
-                                                                                                    cons (mkEqSpec tv1
-                                                                                                          ty2) nil
-                                                                                                | pair _ (Some tv2) =>
-                                                                                                    cons (mkEqSpec tv2
-                                                                                                          ty1) nil
-                                                                                                | _ => nil
-                                                                                                end) else
-                                                                  nil
-                                                              | _ => nil
-                                                              end in
-                                                            Coq.Lists.List.flat_map cont_7__ (GHC.Base.map
-                                                                                     Type.splitTyConApp_maybe theta))).
-
-Definition isLegacyPromotableDataCon : DataCon -> bool :=
-  fun dc =>
-    andb (Data.Foldable.null (dataConEqSpec dc)) (andb (Data.Foldable.null
-                                                        (dataConTheta dc)) (andb (negb (TyCon.isFamInstTyCon
-                                                                                        (dataConTyCon dc)))
-                                                                                 (UniqSet.uniqSetAll
-                                                                                  isLegacyPromotableTyCon
-                                                                                  (Type.tyConsOfType (dataConUserType
-                                                                                                      dc))))).
-
-Definition promoteDataCon : DataCon -> unit :=
+Definition promoteDataCon : DataCon -> TyCon.TyCon :=
   fun arg_0__ =>
     let 'MkData _ _ _ _ _ _ _ _ _ _ _ _ _ _ _ _ _ _ _ _ _ tc := arg_0__ in
     tc.
 
-Definition substEqSpec : TyCoRep.TCvSubst -> EqSpec -> EqSpec :=
-  fun arg_0__ arg_1__ =>
-    match arg_0__, arg_1__ with
-    | subst, Mk_EqSpec tv ty =>
-        let tv' :=
-          Type.getTyVar (GHC.Base.hs_string__ "substEqSpec") (TyCoRep.substTyVar subst
-                                                              tv) in
-        Mk_EqSpec tv' (TyCoRep.substTy subst ty)
-    end.
-
 (* External variables:
-     None Some andb bool cons enumFrom false id list negb nil op_zt__ option orb pair
-     promoted rep_arg_tys rep_ty tag true unit BasicTypes.Arity BasicTypes.ConTag
-     BasicTypes.ConTagZ BasicTypes.SourceText BasicTypes.fIRST_TAG Class.Class
-     Class.classTyCon CoAxiom.Nominal CoAxiom.Representational CoAxiom.Role
-     Coercion.coercionType Coq.Init.Datatypes.app Coq.Lists.List.flat_map
-     Data.Foldable.all Data.Foldable.concatMap Data.Foldable.find
-     Data.Foldable.length Data.Foldable.null Data.Set.Internal.fromList
-     Data.Traversable.mapAccumL Data.Tuple.fst FastString.mkFastString
+     None Some bool false list negb op_zt__ option pair true unit BasicTypes.Arity
+     BasicTypes.ConTag BasicTypes.ConTagZ BasicTypes.SourceText BasicTypes.fIRST_TAG
+     Coq.Init.Datatypes.app Data.Foldable.all Data.Foldable.find Data.Tuple.fst
      FieldLabel.FieldLabel FieldLabel.FieldLabelString FieldLabel.flLabel
-     ForeignCall.CType GHC.Base.Eq_ GHC.Base.const GHC.Base.map GHC.Base.mappend
-     GHC.Base.op_z2218U__ GHC.Base.op_zeze__ GHC.Base.op_zsze__ GHC.Err.Build_Default
-     GHC.Err.Default GHC.Err.error GHC.List.filter GHC.List.replicate GHC.List.zip
-     GHC.Num.fromInteger GHC.Num.op_zm__ GHC.Show.show ListSetOps.assoc Name.Name
-     Name.getName Name.getOccName Name.mkSystemName Name.nameUnique OccName.OccSet
-     OccName.elemOccSet OccName.mkOccSet OccName.mkTyVarOccFS
-     Outputable.assertPprPanic Outputable.op_zdzd__ Panic.assertPanic Panic.noString
-     Panic.panic Panic.panicStr PrelNames.eqTyConKey PrelNames.heqTyConKey
-     TyCoRep.AnId TyCoRep.TCvSubst TyCoRep.mkForAllTys TyCoRep.mkFunTys
-     TyCoRep.mkTyVarTy TyCoRep.mkTyVarTys TyCoRep.substTheta TyCoRep.substTy
-     TyCoRep.substTyVar TyCoRep.substTyVarBndr TyCoRep.substTyWith TyCoRep.substTys
-     TyCoRep.zipTvSubst TyCon.AlgTyConFlav TyCon.AlgTyConRhs TyCon.RuntimeRepInfo
-     TyCon.TyConBinder TyCon.TyConRepName TyCon.isDataProductTyCon_maybe
-     TyCon.isFamInstTyCon TyCon.isFunTyCon TyCon.isKindTyCon TyCon.isTupleTyCon
-     TyCon.isUnboxedSumTyCon TyCon.isUnboxedTupleTyCon TyCon.isVanillaAlgTyCon
-     TyCon.mkAlgTyCon TyCon.mkAnonTyConBinder TyCon.mkNamedTyConBinder
-     TyCon.mkPromotedDataCon TyCon.mkSynonymTyCon TyCon.tyConDataCons
-     TyCon.tyConFamInst_maybe Type.ClassPred Type.EqPred Type.NomEq
-     Type.classifyPredType Type.eqType Type.getTyVar Type.getTyVar_maybe
-     Type.isFamFreeTy Type.isTauTy Type.isTyVarTy Type.mkInvForAllTys
-     Type.mkPrimEqPred Type.mkTyConApp Type.mkTyConBindersPreferAnon
-     Type.splitTyConApp_maybe Type.tyConsOfType TysWiredIn.liftedTypeKind
-     Unify.typesCantMatch UniqSet.UniqSet UniqSet.elementOfUniqSet UniqSet.mkUniqSet
-     UniqSet.uniqSetAll Unique.Unique Unique.getUnique Unique.hasKey
-     Unique.mkAlphaTyVarUnique Util.debugIsOn Util.equalLength Var.Id Var.TvBndr
-     Var.TyVar Var.TyVarBinder Var.binderVars Var.mkTyVar
+     GHC.Base.Eq_ GHC.Base.op_z2218U__ GHC.Base.op_zeze__ GHC.Base.op_zeze____
+     GHC.Base.op_zsze__ GHC.Base.op_zsze____ GHC.Err.Build_Default GHC.Err.Default
+     GHC.Err.error GHC.List.filter GHC.List.replicate GHC.List.zip
+     GHC.Num.fromInteger GHC.Num.op_zm__ Name.Name Name.NamedThing Name.getName__
+     Name.getOccName__ Name.nameOccName OccName.OccName TyCon.TyCon
+     TyCon.isTupleTyCon TyCon.isUnboxedSumTyCon TyCon.isUnboxedTupleTyCon
+     Unique.Uniquable Unique.Unique Unique.getUnique Unique.getUnique__ Var.Id
+     Var.TyVar Var.TyVarBinder Var.binderVars
 *)
